Refactor modules for Cava monad kernel
Signed-off-by: Satnam Singh <satnam@google.com>

cava/cava/Cava/Monad/NetlistGeneration.v
@@ -14,75 +14,18 @@
 (* limitations under the License.                                           *)
 (****************************************************************************)
 
-(* A codification of the Lava embedded DSL develope for Haskell into
-   Coq for the specification, implementaiton and formal verification of circuits.
-   Experimental work, very much in flux, as Satnam learns Coq!
-*)
-
-Require Import Program.Basics.
-From Coq Require Import Bool.Bool.
 From Coq Require Import Ascii String.
-From Coq Require Numbers.BinNums.
-From Coq Require Import ZArith.
-From Coq Require Import Vector.
-From Coq Require Import Bool.Bvector.
 From Coq Require Import Lists.List.
 Import ListNotations.
-
 Require Import ExtLib.Structures.Monads.
-Require Import ExtLib.Structures.MonadFix.
-Require Export ExtLib.Data.Monads.IdentityMonad.
-Require Export ExtLib.Data.Monads.StateMonad.
 Export MonadNotation.
 
-Require Import Cava.Netlist.
-Require Import Cava.Types.
-Require Import Cava.BitArithmetic.
+From Coq Require Import ZArith.
+
+Require Import Cava.Cava.
+Require Import Cava.Monad.CavaClass.
+
 Require Import Cava.Signal.
-
-Generalizable All Variables.
-
-Local Open Scope list_scope.
-Local Open Scope monad_scope.
-Local Open Scope string_scope.
-
-(* The Cava class represents circuit graphs with Coq-level inputs and
-   outputs, but does not represent the IO ports of circuits. This allows
-   us to define both circuit netlist interpretations for the Cava class
-   as well as behavioural interpretations for attributing semantics. *)
-Class Cava m bit `{Monad m} := {
-  (* Constant values. *)
-  zero : m bit; (* This component always returns the value 0. *)
-  one : m bit; (* This component always returns the value 1. *)
-  delayBit : bit -> m bit; (* Cava bit-level unit delay. *)
-  loopBit : forall {A B : Type}, ((A * bit)%type -> m (B * bit)%type) -> A -> m B;
-  (* Primitive gates *)
-  inv : bit -> m bit;
-  and2 : bit * bit -> m bit;
-  nand2 : bit * bit -> m bit;
-  or2 : bit * bit -> m bit;
-  nor2 : bit * bit -> m bit;
-  xor2 : bit * bit -> m bit;
-  xnor2 : bit * bit -> m bit;
-  buf_gate : bit -> m bit; (* Corresponds to the SystemVerilog primitive gate 'buf' *)
-  (* Xilinx UNISIM FPGA gates *)
-  lut1 : (bool -> bool) -> bit -> m bit; (* 1-input LUT *)
-  lut2 : (bool -> bool -> bool) -> (bit * bit) -> m bit; (* 2-input LUT *)
-  lut3 : (bool -> bool -> bool -> bool) -> (bit * bit * bit) -> m bit; (* 3-input LUT *)
-  lut4 : (bool -> bool -> bool -> bool -> bool) -> (bit * bit * bit * bit) ->
-         m bit; (* 4-input LUT *)
-  lut5 : (bool -> bool -> bool -> bool -> bool -> bool) ->
-         (bit * bit * bit * bit * bit) -> m bit; (* 5-input LUT *)
-  lut6 : (bool -> bool -> bool -> bool -> bool -> bool -> bool) ->
-         (bit * bit * bit * bit * bit * bit) -> m bit; (* 6-input LUT *)
-  xorcy : bit * bit -> m bit; (* Xilinx fast-carry UNISIM with arguments O, CI, LI *)
-  muxcy : bit -> bit -> bit -> m bit; (* Xilinx fast-carry UNISIM with arguments O, CI, DI, S *)
-  (* Synthesizable multiplexors *)
-  indexBitArray : list bit -> list bit -> m bit;
-  indexArray : list (list bit) -> list bit -> m (list bit);
-  (* Synthesizable arithmetic operations. *)
-  unsignedAdd : list bit -> list bit -> m (list bit);
-}.
 
 (******************************************************************************)
 (* Netlist implementations for the Cava class.                                *)
@@ -307,125 +250,3 @@ Instance CavaNet : Cava (state CavaState) Signal :=
     indexArray := indexArrayNet;
     unsignedAdd := unsignedAddNet;
 }.
-
-(******************************************************************************)
-(* A second boolean combinational logic interpretation for the Cava class     *)
-(******************************************************************************)
-
-Definition notBool (i: bool) : ident bool :=
-  ret (negb i).
-
-Definition andBool '(a, b) : ident bool :=
-  ret (a && b).
-
-Definition nandBool (i: bool * bool) : ident bool :=
-  let (a, b) := i in ret (negb (a && b)).
-
-Definition orBool (i: bool * bool) : ident bool :=
-  let (a, b) := i in ret (a || b).
-
-Definition norBool (i: bool * bool) : ident bool :=
-  let (a, b) := i in ret (negb (a || b)).
-
-Definition xorBool (i: bool * bool) : ident bool :=
-  let (a, b) := i in ret (xorb a b).
-
-Definition xnorBool (i : bool * bool) : ident bool :=
-  let (a, b) := i in ret (negb (xorb a b)).
-
-Definition lut1Bool (f: bool -> bool) (i: bool) : ident bool := ret (f i).
-
-Definition lut2Bool (f: bool -> bool -> bool) (i: bool * bool) : ident bool :=
-  ret (f (fst i) (snd i)).
-
-Definition lut3Bool (f: bool -> bool -> bool -> bool) (i: bool * bool * bool) :
-                    ident bool :=
-  let '(i0, i1, i2) := i in
-  ret (f i0 i1 i2).
-
-Definition lut4Bool (f: bool -> bool -> bool -> bool -> bool)
-                    (i: bool * bool * bool * bool) : ident bool :=
-  let '(i0, i1, i2, i3) := i in
-  ret (f i0 i1 i2 i3).
-
-Definition lut5Bool (f: bool -> bool -> bool -> bool -> bool -> bool)
-                    (i: bool * bool * bool * bool * bool) : ident bool :=
-  let '(i0, i1, i2, i3, i4) := i in
-  ret (f i0 i1 i2 i3 i4).
-
-Definition lut6Bool (f: bool -> bool -> bool -> bool -> bool -> bool -> bool)
-                    (i: bool * bool * bool * bool * bool * bool) : ident bool :=
-  let '(i0, i1, i2, i3, i4, i5) := i in
-  ret (f i0 i1 i2 i3 i4 i5).
-
-Definition xorcyBool (i: bool * bool) : ident bool :=
-  let (ci, li) := i in ret (xorb ci li).
-
-Definition muxcyBool (s : bool) (ci : bool) (di : bool) : ident bool :=
-  ret (match s with
-       | false => di
-       | true => ci
-       end).
-
-Definition indexBitArrayBool (i : list bool) (sel : list bool) :
-                             ident bool :=
-  let selNat := list_bits_to_nat sel in
-  ret (nth (N.to_nat selNat) i false).
-
-Definition indexArrayBool (i : list (list bool)) (sel : list bool) :
-                             ident (list bool) :=
-  let selNat := list_bits_to_nat sel in
-  ret (nth (N.to_nat selNat) i []).
-
-Definition unsignedAddBool (av : list bool) (bv : list bool) :
-                           ident (list bool) :=
-  let a := list_bits_to_nat av in
-  let b := list_bits_to_nat bv in
-  let sumSize := max (length av) (length bv) + 1 in
-  let sum := (a + b)%N in
-  ret (nat_to_list_bits_sized sumSize sum).
-
-Definition bufBool (i : bool) : ident bool :=
-  ret i.
-
-Definition loopBitBool (A B : Type) (f : A * bool -> ident (B * bool)) (a : A) : ident B :=
-  '(b, _) <- f (a, false) ;;
-  ret b.
-
-(******************************************************************************)
-(* Instantiate the Cava class for a boolean combinational logic               *)
-(* interpretation.                                                            *)
-(******************************************************************************)
-
-Instance CavaBool : Cava ident bool :=
-  { zero := ret false;
-    one := ret true;
-    delayBit i := ret i; (* Dummy definition for delayBit for now. *)
-    loopBit a b := loopBitBool a b;
-    inv := notBool;
-    and2 := andBool;
-    nand2 := nandBool;
-    or2 := orBool;
-    nor2 := norBool;
-    xor2 := xorBool;
-    lut1 := lut1Bool;
-    lut2 := lut2Bool;
-    lut3 := lut3Bool;
-    lut4 := lut4Bool;
-    lut5 := lut5Bool;
-    lut6 := lut6Bool;
-    xorcy := xorcyBool;
-    xnor2 := xnorBool;
-    muxcy := muxcyBool;
-    indexBitArray := indexBitArrayBool;
-    indexArray := indexArrayBool;
-    unsignedAdd m n := @unsignedAddBool m n;
-    buf_gate := bufBool;
-}.
-
-(******************************************************************************)
-(* A function to run a monadic circuit description and return the boolean     *)
-(* behavioural simulation result.                                             *)
-(******************************************************************************)
-
-Definition combinational {a} (circuit : ident a) : a := unIdent circuit.
