cava/cava/Cava/Monad/CavaClass.v
@@ -1,0 +1,55 @@
+(****************************************************************************)
+(* Copyright 2020 The Project Oak Authors                                   *)
+(*                                                                          *)
+(* Licensed under the Apache License, Version 2.0 (the "License")           *)
+(* you may not use this file except in compliance with the License.         *)
+(* You may obtain a copy of the License at                                  *)
+(*                                                                          *)
+(*     http://www.apache.org/licenses/LICENSE-2.0                           *)
+(*                                                                          *)
+(* Unless required by applicable law or agreed to in writing, software      *)
+(* distributed under the License is distributed on an "AS IS" BASIS,        *)
+(* WITHOUT WARRANTIES OR CONDITIONS OF ANY KIND, either express or implied. *)
+(* See the License for the specific language governing permissions and      *)
+(* limitations under the License.                                           *)
+(****************************************************************************)
+
+Require Import ExtLib.Structures.Monads.
+
+(* The Cava class represents circuit graphs with Coq-level inputs and
+   outputs, but does not represent the IO ports of circuits. This allows
+   us to define both circuit netlist interpretations for the Cava class
+   as well as behavioural interpretations for attributing semantics. *)
+Class Cava m bit `{Monad m} := {
+  (* Constant values. *)
+  zero : m bit; (* This component always returns the value 0. *)
+  one : m bit; (* This component always returns the value 1. *)
+  delayBit : bit -> m bit; (* Cava bit-level unit delay. *)
+  loopBit : forall {A B : Type}, ((A * bit)%type -> m (B * bit)%type) -> A -> m B;
+  (* Primitive gates *)
+  inv : bit -> m bit;
+  and2 : bit * bit -> m bit;
+  nand2 : bit * bit -> m bit;
+  or2 : bit * bit -> m bit;
+  nor2 : bit * bit -> m bit;
+  xor2 : bit * bit -> m bit;
+  xnor2 : bit * bit -> m bit;
+  buf_gate : bit -> m bit; (* Corresponds to the SystemVerilog primitive gate 'buf' *)
+  (* Xilinx UNISIM FPGA gates *)
+  lut1 : (bool -> bool) -> bit -> m bit; (* 1-input LUT *)
+  lut2 : (bool -> bool -> bool) -> (bit * bit) -> m bit; (* 2-input LUT *)
+  lut3 : (bool -> bool -> bool -> bool) -> (bit * bit * bit) -> m bit; (* 3-input LUT *)
+  lut4 : (bool -> bool -> bool -> bool -> bool) -> (bit * bit * bit * bit) ->
+         m bit; (* 4-input LUT *)
+  lut5 : (bool -> bool -> bool -> bool -> bool -> bool) ->
+         (bit * bit * bit * bit * bit) -> m bit; (* 5-input LUT *)
+  lut6 : (bool -> bool -> bool -> bool -> bool -> bool -> bool) ->
+         (bit * bit * bit * bit * bit * bit) -> m bit; (* 6-input LUT *)
+  xorcy : bit * bit -> m bit; (* Xilinx fast-carry UNISIM with arguments O, CI, LI *)
+  muxcy : bit -> bit -> bit -> m bit; (* Xilinx fast-carry UNISIM with arguments O, CI, DI, S *)
+  (* Synthesizable multiplexors *)
+  indexBitArray : list bit -> list bit -> m bit;
+  indexArray : list (list bit) -> list bit -> m (list bit);
+  (* Synthesizable arithmetic operations. *)
+  unsignedAdd : list bit -> list bit -> m (list bit);
+}.
