cava/cava/Cava/Monad/CombinationalMonad.v
@@ -1,0 +1,150 @@
+(****************************************************************************)
+(* Copyright 2020 The Project Oak Authors                                   *)
+(*                                                                          *)
+(* Licensed under the Apache License, Version 2.0 (the "License")           *)
+(* you may not use this file except in compliance with the License.         *)
+(* You may obtain a copy of the License at                                  *)
+(*                                                                          *)
+(*     http://www.apache.org/licenses/LICENSE-2.0                           *)
+(*                                                                          *)
+(* Unless required by applicable law or agreed to in writing, software      *)
+(* distributed under the License is distributed on an "AS IS" BASIS,        *)
+(* WITHOUT WARRANTIES OR CONDITIONS OF ANY KIND, either express or implied. *)
+(* See the License for the specific language governing permissions and      *)
+(* limitations under the License.                                           *)
+(****************************************************************************)
+
+From Coq Require Import Bool.Bool.
+From Coq Require Import Ascii String.
+From Coq Require Import Lists.List.
+Import ListNotations.
+Require Import ExtLib.Structures.Monads.
+Require Export ExtLib.Data.Monads.IdentityMonad.
+Export MonadNotation.
+
+From Coq Require Import ZArith.
+
+Require Import Cava.Cava.
+Require Import Cava.Monad.CavaClass.
+
+(******************************************************************************)
+(* A boolean combinational logic interpretation for the Cava class            *)
+(******************************************************************************)
+
+Definition notBool (i: bool) : ident bool :=
+  ret (negb i).
+
+Definition andBool '(a, b) : ident bool :=
+  ret (a && b).
+
+Definition nandBool (i: bool * bool) : ident bool :=
+  let (a, b) := i in ret (negb (a && b)).
+
+Definition orBool (i: bool * bool) : ident bool :=
+  let (a, b) := i in ret (a || b).
+
+Definition norBool (i: bool * bool) : ident bool :=
+  let (a, b) := i in ret (negb (a || b)).
+
+Definition xorBool (i: bool * bool) : ident bool :=
+  let (a, b) := i in ret (xorb a b).
+
+Definition xnorBool (i : bool * bool) : ident bool :=
+  let (a, b) := i in ret (negb (xorb a b)).
+
+Definition lut1Bool (f: bool -> bool) (i: bool) : ident bool := ret (f i).
+
+Definition lut2Bool (f: bool -> bool -> bool) (i: bool * bool) : ident bool :=
+  ret (f (fst i) (snd i)).
+
+Definition lut3Bool (f: bool -> bool -> bool -> bool) (i: bool * bool * bool) :
+                    ident bool :=
+  let '(i0, i1, i2) := i in
+  ret (f i0 i1 i2).
+
+Definition lut4Bool (f: bool -> bool -> bool -> bool -> bool)
+                    (i: bool * bool * bool * bool) : ident bool :=
+  let '(i0, i1, i2, i3) := i in
+  ret (f i0 i1 i2 i3).
+
+Definition lut5Bool (f: bool -> bool -> bool -> bool -> bool -> bool)
+                    (i: bool * bool * bool * bool * bool) : ident bool :=
+  let '(i0, i1, i2, i3, i4) := i in
+  ret (f i0 i1 i2 i3 i4).
+
+Definition lut6Bool (f: bool -> bool -> bool -> bool -> bool -> bool -> bool)
+                    (i: bool * bool * bool * bool * bool * bool) : ident bool :=
+  let '(i0, i1, i2, i3, i4, i5) := i in
+  ret (f i0 i1 i2 i3 i4 i5).
+
+Definition xorcyBool (i: bool * bool) : ident bool :=
+  let (ci, li) := i in ret (xorb ci li).
+
+Definition muxcyBool (s : bool) (ci : bool) (di : bool) : ident bool :=
+  ret (match s with
+       | false => di
+       | true => ci
+       end).
+
+Definition indexBitArrayBool (i : list bool) (sel : list bool) :
+                             ident bool :=
+  let selNat := list_bits_to_nat sel in
+  ret (nth (N.to_nat selNat) i false).
+
+Definition indexArrayBool (i : list (list bool)) (sel : list bool) :
+                             ident (list bool) :=
+  let selNat := list_bits_to_nat sel in
+  ret (nth (N.to_nat selNat) i []).
+
+Definition unsignedAddBool (av : list bool) (bv : list bool) :
+                           ident (list bool) :=
+  let a := list_bits_to_nat av in
+  let b := list_bits_to_nat bv in
+  let sumSize := max (length av) (length bv) + 1 in
+  let sum := (a + b)%N in
+  ret (nat_to_list_bits_sized sumSize sum).
+
+Definition bufBool (i : bool) : ident bool :=
+  ret i.
+
+Definition loopBitBool (A B : Type) (f : A * bool -> ident (B * bool)) (a : A) : ident B :=
+  '(b, _) <- f (a, false) ;;
+  ret b.
+
+(******************************************************************************)
+(* Instantiate the Cava class for a boolean combinational logic               *)
+(* interpretation.                                                            *)
+(******************************************************************************)
+
+Instance CavaBool : Cava ident bool :=
+  { zero := ret false;
+    one := ret true;
+    delayBit i := ret i; (* Dummy definition for delayBit for now. *)
+    loopBit a b := loopBitBool a b;
+    inv := notBool;
+    and2 := andBool;
+    nand2 := nandBool;
+    or2 := orBool;
+    nor2 := norBool;
+    xor2 := xorBool;
+    lut1 := lut1Bool;
+    lut2 := lut2Bool;
+    lut3 := lut3Bool;
+    lut4 := lut4Bool;
+    lut5 := lut5Bool;
+    lut6 := lut6Bool;
+    xorcy := xorcyBool;
+    xnor2 := xnorBool;
+    muxcy := muxcyBool;
+    indexBitArray := indexBitArrayBool;
+    indexArray := indexArrayBool;
+    unsignedAdd m n := @unsignedAddBool m n;
+    buf_gate := bufBool;
+}.
+
+(******************************************************************************)
+(* A function to run a monadic circuit description and return the boolean     *)
+(* behavioural simulation result.                                             *)
+(******************************************************************************)
+
+Definition combinational {a} (circuit : ident a) : a := unIdent circuit.
