cava/monad-examples/FullAdder.v
@@ -15,26 +15,15 @@
 
 From Coq Require Import Bool.Bool.
 From Coq Require Import Ascii String.
-From Coq Require Import Vector.
-From Coq Require Import Bool.Bvector.
 From Coq Require Import Lists.List.
 Require Import Omega.
 Import ListNotations.
 
-Require Import Nat Arith Lia.
-
 Require Import ExtLib.Structures.Monads.
 
-Require Import Cava.Monad.Cava.
-Require Import Cava.Netlist.
-Require Import Cava.Types.
-Require Import Cava.Monad.Combinators.
-Require Import Cava.BitArithmetic.
+Require Import Cava.Cava.
+Require Import Cava.Monad.CavaMonad.
 Require Import Cava.Monad.XilinxAdder.
-
-Local Open Scope list_scope.
-Local Open Scope monad_scope.
-Local Open Scope string_scope.
 
 (******************************************************************************)
 (* Build a half-adder                                                         *)
@@ -136,6 +125,3 @@ Local Open Scope list_scope.
 Definition adderWithGrowth {m bit} `{Cava m bit} '(cin, (a, b)):=
   '(sum, carryOut) <- adder (cin, (a, b)) ;;
   ret (sum ++ [carryOut]).
-
-
-
